---
title: Fields and Galois Theory, 1
---

## Solution to Exercise 1.4 of Chapter 1

*Prove the equivalence of (R9) and (R9)' (Howie 5).*

**Proof:** For a commutative ring $$R$$ with unity, recall that (R9) and (R9)' are as follows:

(R9) For all $$a$$, $$b$$, $$c$$ in $$R$$ with $$c \neq 0$$,

\begin{equation}
ca = cb \Rightarrow a = b\mbox{.}
\end{equation}

(R9)' For all $$a$$, $$b$$ in $$R$$,

\begin{equation}
ab = 0 \Rightarrow a = 0 \mbox{ or } b = 0\mbox{.}
\end{equation}

(R9) $$\Rightarrow$$ (R9)'. Suppose that $$ab = 0$$ and $$a \neq 0$$ for $$a$$, $$b$$ in $$R$$. Then, 

$$ab = 0 = a0 \Rightarrow b = 0$$

(R9)' $$\Rightarrow$$ (R9). Suppose that $$ca = ba$$ for $$a$$, $$b$$, $$c$$ in $$R$$ with $$c \neq 0$$. Then,

\begin{align}
ca = cb & \Rightarrow ca - cb = 0 \\\\\\
        & \Rightarrow c(a-b) = 0
\end{align}

and $$a - b = 0$$ since $$c \neq 0$$. Therefore $$a = b$$. *Q.E.D.*

## Reference

Howie, John. *Fields and Galois Theory*, Springer, 2005.
