---
title: Elementary Number Theory, 1
---

## Solution to Problem 4 of Section 1

*If $$N = abc + 1$$, prove that $$(N, a) = (N, b) = (N, c) = 1$$ (Dudley 9).*

**Proof:** Suppose that $$a$$, $$b$$ and $$c$$ are positive integers. For $$a$$, by the Euclidean algorihtm,

\begin{align}
N & = a(bc) + 1 \\\\\\
a & = 1 \cdot a
\end{align}

and $$(N, a) = 1$$. Similarly, $$(N, b) = 1$$ and $$(N, c) = 1$$. *Q.E.D.*

## Reference

Dudley, Underwood. *Elementary Number Theory*. Second Edition, Dover Publications, 2008.
